Impl.read_header

src/QUIC.Impl.Header.Parse.fst
@@ -184,3 +184,147 @@ let putative_pn_offset
   else Some res
 
 #pop-options
+
+let impl_protected_bits_pn_length
+  (is_short: bool)
+  (pb: secret_bitfield (if is_short then 5 else 4))
+: Tot (y: PN.packet_number_length_t { y == protected_bits_pn_length is_short (Secret.reveal pb) })
+= Secret.to_u32 #Secret.U8 (Secret.to_u8 1uy `Secret.add` Secret.get_bitfield #Secret.U8 pb 0ul 2ul)
+
+let impl_protected_bits_reserved
+  (is_short: bool)
+  (pb: secret_bitfield (if is_short then 5 else 4))
+: Tot (y: secret_bitfield 2 { Secret.reveal y == protected_bits_reserved is_short (Secret.reveal pb) })
+= if is_short
+  then Secret.get_bitfield #Secret.U8 pb 3ul 5ul
+  else Secret.get_bitfield #Secret.U8 pb 2ul 4ul
+
+let impl_protected_bits_key_phase
+  (x: secret_bitfield 5)
+: Tot (y: secret_bitfield 1 { protected_bits_key_phase (Secret.reveal x) == (Secret.v y = 1) })
+= Secret.get_bitfield #Secret.U8 x 2ul 3ul
+
+let header_p
+  (h: Public.header)
+: Tot header
+= match h with
+  | Public.PShort pb spin cid cid_len ->
+    let rb = impl_protected_bits_reserved true pb in
+    let phase = impl_protected_bits_key_phase pb in
+    let pnl = impl_protected_bits_pn_length true pb in
+    BShort rb spin phase cid cid_len pnl
+  | Public.PLong pb version dcid dcil scid scil spec ->
+    let rb = impl_protected_bits_reserved false pb in
+    let pnl = impl_protected_bits_pn_length false pb in
+    BLong version dcid dcil scid scil
+    begin match spec with
+    | Public.PInitial payload_and_pn_length token token_length ->
+      BInitial rb payload_and_pn_length pnl token token_length
+    | Public.PHandshake payload_and_pn_length ->
+      BHandshake rb payload_and_pn_length pnl
+    | Public.PZeroRTT payload_and_pn_length ->
+      BZeroRTT rb payload_and_pn_length pnl
+    | Public.PRetry odcid odcil ->
+      BRetry pb odcid odcil
+    end
+
+#push-options "--z3rlimit 16"
+
+let g_header_header_p
+  (cid_len: short_dcid_len_t)
+  (last: PN.last_packet_number_t)
+  (m: HS.mem)
+  (ph: Public.header { Public.parse_header_prop cid_len (Public.g_header ph m) })
+  (pn: PN.packet_number_t)
+: Lemma (
+    let h = header_p ph in
+    let gh = Public.g_header ph m in
+    if
+      if Public.is_retry ph
+      then true
+      else
+        let pn_len = pn_length h in
+        PN.in_window (Secret.v pn_len - 1) (Secret.v last) (Secret.v pn)
+    then
+      let h' = synth_header cid_len last (| gh, (if Public.is_retry ph then () else pn) |) in
+      g_header (header_p ph) m pn == h'
+    else
+      True
+  )
+= ()
+
+#pop-options
+
+let parse_public_header_consumes
+  (cid_len: short_dcid_len_t)
+  (x: bytes)
+  (ph: Public.header)
+  (m: HS.mem)
+: Lemma
+  (requires (
+    match LP.parse (Public.parse_header cid_len) x with
+    | None -> False
+    | Some (ph0, _) -> Public.g_header ph m == ph0
+  ))
+  (ensures (
+    let Some (ph0, consumed) = LP.parse (Public.parse_header cid_len) x in
+    consumed == U32.v (Public.header_len ph)
+  ))
+= let Some (ph0, consumed) = LP.parse (Public.parse_header cid_len) x in
+  Public.header_len_correct cid_len m ph;
+  LP.parse_serialize (Public.serialize_header cid_len) ph0;
+  LP.parse_injective (Public.parse_header cid_len) x (LP.serialize (Public.serialize_header cid_len) ph0)
+
+let public_header_len_complete
+  (h: Public.header)
+: Lemma
+  (public_header_len (header_p h) == Public.header_len h)
+= ()
+
+#push-options "--z3rlimit 64"
+
+let read_header
+  packet packet_len cid_len last
+=
+  let m = HST.get () in
+  assert (Some? (Spec.putative_pn_offset (U32.v cid_len) (B.as_seq m packet)));
+  parse_header_exists (U32.v cid_len) (Secret.v last) (B.as_seq m packet);
+  lp_parse_header_eq cid_len last (B.as_seq m packet);
+  let ph = Public.read_header packet packet_len cid_len in
+  let m1 = HST.get () in
+  public_header_len_complete ph;
+  parse_public_header_consumes cid_len (B.as_seq m packet) ph m1;
+  let h = header_p ph in
+  if Public.is_retry ph
+  then begin
+    g_header_header_p cid_len last m ph last;
+    (h, last)
+  end else begin
+    let len = Public.header_len ph in
+    LP.parsed_data_is_serialize (Public.serialize_header cid_len) (B.as_seq m packet);
+    assert (Seq.index (B.as_seq m packet) 0 == Seq.index (LP.serialize (Public.serialize_header cid_len) (Public.g_header ph m1)) 0);
+    Public.serialize_header_is_retry cid_len (Public.g_header ph m1);
+    assert (U32.v len + 4 <= B.length packet);
+    let pn_len = pn_length h in
+    let pn = SecretBuffer.with_buffer_hide
+      #PN.packet_number_t
+      packet
+      len
+      packet_len
+      m1
+      B.loc_none
+      B.loc_none
+      0ul 0ul 0ul 0ul 0ul 0ul
+      (fun pn _ cont _ _ ->
+        match LP.parse (PN.parse_packet_number last pn_len) cont with
+        | None -> False
+        | Some (pn', _) -> pn == pn'
+      )
+      (fun _ _ bs _ ->
+        PN.read_packet_number last pn_len bs
+      )
+    in
+    (h, pn)
+  end
+
+#pop-options
